

$$u = \begin{pmatrix} \tau_\phi \\ \tau_\theta \\ \tau_\psi \end{pmatrix}, \quad y_{\text{out}} = \begin{pmatrix} x \\ y \\ z \end{pmatrix}$$

$$\xi = (x, y, z, V_x^b, V_y^b, V_z^b, \phi, \theta, \psi, p, q, r)$$

$$\dot{\xi} = \begin{pmatrix} \dot{p} \\ \dot{q} \\ \dot{r} \\ \dot{\omega} \end{pmatrix} = \begin{pmatrix} \frac{1}{m} [F_{\text{thrust}}^b + F_{\text{gravity}}^b + F_{\text{drag}}^b] - \omega \times V^b \\ W(\omega) \omega \\ I^{-1} (\tau_{\text{control}}^b + \tau_{\text{drag}}^b - \omega \times I \omega) \end{pmatrix}$$

$$\text{yaw} \quad \dot{q}_4 = \dot{\psi} = \frac{\sin \phi}{\cos \theta} q + \frac{\cos \phi}{\cos \theta} r$$

$$\ddot{q}_4 = \ddot{\psi} = \underbrace{(s_\phi \sec \theta) \dot{q} + (c_\phi \sec \theta) \dot{r}}_{\text{input-dependent part}} + \underbrace{(\dot{\phi} c_\phi \sec \theta + s_\phi \dot{\theta} \sec \theta \tan \theta) q + (-\dot{\phi} s_\phi \sec \theta + c_\phi \dot{\theta} \sec \theta \tan \theta) r}_{\text{state-dependent part } f_\psi(\xi) \text{ [drift]}}$$

$$\rightarrow \begin{pmatrix} 0 & s_\phi \sec \theta & c_\phi \sec \theta \end{pmatrix} \begin{pmatrix} \dot{p} \\ \dot{q} \\ \dot{r} \end{pmatrix}$$

$$\dot{\omega} = I^{-1} [\tau_{\text{tot}}^b - \omega \times I \omega]$$

$$= L_\psi(\xi) + (0 \quad s_\phi \sec \theta \quad c_\phi \sec \theta) I^{-1} [\tau_{\text{tot}}^b - \omega \times I \omega] = f_\psi(\xi) + (0 \quad s_\phi \sec \theta \quad c_\phi \sec \theta) I^{-1} \left[\begin{pmatrix} \tau_\phi \\ \tau_\theta \\ \tau_\psi \end{pmatrix} - A_{\text{rot}} \omega - \omega \times I \omega \right]$$

$$\rightarrow \tau_{\text{control}}^b + \tau_{\text{drag}}^b = \begin{pmatrix} \tau_\phi \\ \tau_\theta \\ \tau_\psi \end{pmatrix} - A_{\text{rot}} \omega$$

$$\Rightarrow \ddot{\psi} = f_\psi(\xi) + g_{\psi, \phi}(\xi) \tau_\phi + g_{\psi, \theta}(\xi) \tau_\theta + g_{\psi, \psi}(\xi) \tau_\psi = F(\xi) + G(\xi) u$$

position

$$\dot{P} = R(\theta) V^b = f(V^b, \theta) = f(\phi, \theta, \psi, V_x^b, V_y^b, V_z^b) \text{ function of the state}$$

$$\ddot{P} = \dot{R} V^b + R \dot{V}^b = \underbrace{R S(\omega)}_{\text{RS}(\omega)} V^b + \underbrace{R \left(\frac{1}{m} (F_{\text{thrust}}^b + F_{\text{gravity}}^b + F_{\text{drag}}^b) - \omega \times V^b \right)}_{R(\omega \times V^b)} = \frac{1}{m} R \begin{pmatrix} 0 \\ 0 \\ F_T \end{pmatrix} + \begin{pmatrix} 0 \\ 0 \\ -g \end{pmatrix} - \frac{1}{m} A_{\text{trans}} V^b$$

$$P^{(3)} = \frac{d}{dt} \left[\underbrace{\frac{F_T}{m} R \begin{pmatrix} 0 \\ 0 \\ 1 \end{pmatrix}}_{\text{1}} + \underbrace{\begin{pmatrix} 0 \\ 0 \\ -g \end{pmatrix}}_{\text{2}} + \underbrace{\frac{1}{m} R F_{\text{drag}}^b}_{\text{3}} \right] = \frac{\dot{F}_T}{m} R e_3 + \frac{F_T}{m} R S(\omega) e_3 + \frac{1}{m} [\dot{R} F_{\text{drag}}^b + R \dot{F}_{\text{drag}}^b]$$

$$\textcircled{2} \quad \frac{d}{dt} \left[\frac{F_T}{m} R \begin{pmatrix} 0 \\ 0 \\ 1 \end{pmatrix} \right] = \underbrace{\frac{\dot{F}_T}{m} R \begin{pmatrix} 0 \\ 0 \\ 1 \end{pmatrix}}_{\text{not a control}} + \frac{F_T}{m} \dot{R} \begin{pmatrix} 0 \\ 0 \\ 1 \end{pmatrix}$$

\Rightarrow define dynamic compensator
state $\zeta_1 = F_T \Rightarrow \dot{\zeta}_1 = \dot{F}_T = \underbrace{v_T}_{\text{new input}}$

$$\textcircled{2} \quad \frac{d}{dt} \left[\begin{pmatrix} 0 \\ -g \end{pmatrix} = \text{const} \right] = 0$$

$$\textcircled{3} \quad \frac{d}{dt} \left[\frac{1}{m} R F_{\text{drag}}^b \right] = \frac{1}{m} [\underbrace{\dot{R} F_{\text{drag}}^b}_{R(\omega \times F_{\text{drag}}^b)} + \underbrace{R \dot{F}_{\text{drag}}^b}_{\text{contains } \dot{V}_b}] = \frac{1}{m} [R(\omega \times F_{\text{drag}}^b) - R A_{\text{trans}} \left(\frac{1}{m} (F_{\text{thrust}}^b + F_{\text{gravity}}^b + F_{\text{drag}}^b) - \omega \times V^b \right)]$$

\rightarrow does not introduce any new input

$$P^{(u)} = \frac{d}{dt} \left[\underbrace{\frac{\dot{F}_T}{m} R e_3}_{\text{1}} + \underbrace{\frac{F_T}{m} R S(\omega) e_3}_{\text{2}} + \dots \right]$$

$$\textcircled{1} \quad \frac{d}{dt} \left[\frac{\dot{F}_T}{m} R e_3 \right] = \underbrace{\frac{\ddot{F}_T}{m} R e_3}_{\zeta_2 = \ddot{F}_T \Rightarrow \dot{\zeta}_2 = \ddot{F}_T = \underbrace{v_T}_{\text{new input}}} + \frac{\dot{F}_T}{m} \dot{R} e_3$$

$$\textcircled{2} \quad \frac{d}{dt} \left[\frac{F_T}{m} R S(\omega) e_3 \right] = \frac{\dot{F}_T}{m} R S(\omega) e_3 + \frac{F_T}{m} \dot{R} S(\omega) e_3 + \frac{F_T}{m} \underbrace{R S(\dot{\omega}) e_3}_{\dot{\omega} \times e_3}$$

$$I^{-1} (\tau_{\text{control}}^b + \tau_{\text{drag}}^b - \omega \times I \omega) \rightarrow \begin{pmatrix} \tau_\phi \\ \tau_\theta \\ \tau_\psi \end{pmatrix}$$

$$\Rightarrow \begin{pmatrix} P^{(u)} \\ \ddot{\psi} \end{pmatrix} = J(\xi, \zeta) \tilde{u} + l(\xi, \zeta)$$

$$\Rightarrow \tilde{u} = J^{-1}(\xi, \zeta) [v - l(\xi, \zeta)] \leftarrow \text{linearizing feedback law}$$

$$\begin{matrix} \begin{pmatrix} \ddot{F}_T \\ \tau_\phi \\ \tau_\theta \\ \tau_\psi \end{pmatrix} & \begin{pmatrix} v_1 \\ v_2 \\ v_3 \\ v_4 \end{pmatrix} \end{matrix}$$

linearized system \rightarrow

$$\begin{aligned} x^{(u)} &= v_1 \\ y^{(u)} &= v_2 \\ z^{(u)} &= v_3 \\ \ddot{\psi} &= v_4 \end{aligned}$$

$$r = r_x + r_y + r_z + r_\psi = 4 + 4 + 4 + 2 = 14$$

$$\begin{matrix} n = 12 \\ v = 2 \\ m = 4 \end{matrix} \left. \vphantom{\begin{matrix} n \\ v \\ m \end{matrix}} \right\} n_{\text{ext}} = 12 + 2 = 14 \Rightarrow r = n_{\text{ext}} \Rightarrow \text{fully state linearizable}$$